Okay this fails

Dpda/Definition/Sipser.lean
@@ -33,6 +33,87 @@ structure Sipser_DPDA_IDesc (Q) (S) (Γ) where
   w : List S
   β : List Γ
 
+
+-- This is the version that does not depend on the `deterministic` condition.
+-- This is intended as a workaround in Lean's `motive is not type correct` error.
+def Sipser_PreDPDA.stepTransition {Q S Γ}
+  (M: Sipser_PreDPDA Q S Γ)
+  (pwβ: Sipser_DPDA_IDesc Q S Γ)
+  : Option (Sipser_DPDA_IDesc Q S Γ) :=
+  /-
+
+  A Sipser DPDA has exactly one legal move in every situation where its stack is nonempty.
+  If the stack is empty, a Sipser DPDA can move only if the transition function specifies a move that pops ε.
+  -/
+
+  match M.transition (pwβ.p, AugmentEpsilon.Epsilon, AugmentEpsilon.Epsilon) with
+  | some (r, y) =>
+    -- If δ(q, ε, ε) is nonempty, there is no restriction on the input or stack.
+    -- · move to the state r,
+    -- · consume nothing from the input
+    -- · pop nothing from the stack
+    -- · push y onto the stack
+    some ⟨ r, pwβ.w, y.toList ++ pwβ.β ⟩
+  | none =>
+    -- Otherwise, ∀ a x, exactly one of δ(q, a, x), δ(q, ε, x), or δ(q, a, ε) is `some`.
+    -- Thus we first need to check whether the stack or the input is empty.
+    match pwβ.w, pwβ.β with
+    | [], [] =>
+      -- If both the input and the stack are empty, we cannot move,
+      -- since the only potential legal move, δ(q, ε, ε), turned out to be empty.
+      none
+    | [], x :: xs =>
+      -- We cannot consume from an empty input, so our only hope is δ(q, ε, x), a transition without the input consumption.
+      match M.transition (pwβ.p, AugmentEpsilon.Epsilon, AugmentEpsilon.fromChar x) with
+      | some (r, y) =>
+        -- If δ(q, ε, x) is nonempty, we can pop x from the stack,
+        -- move to the state r,
+        -- consume nothing from the input,
+        -- and push y onto the stack.
+        some ⟨ r, pwβ.w, y.toList ++ xs ⟩
+      | none =>
+        -- If δ(q, ε, x) is empty, we cannot move.
+        none
+    | a :: ws, [] =>
+      -- If the stack is empty, our only legal option is δ(q, a, ε), a transition without the stack pop.
+      match M.transition (pwβ.p, AugmentEpsilon.fromChar a, AugmentEpsilon.Epsilon) with
+      | some (r, y) =>
+        -- If δ(q, a, ε) is nonempty, we can consume a from the input,
+        -- move to the state r,
+        -- pop nothing from the stack,
+        -- and push y onto the stack.
+        some ⟨ r, ws, y.toList ++ pwβ.β ⟩
+      | none =>
+        -- If δ(q, a, ε) is empty, we cannot move.
+        none
+    | a :: ws, x :: xs =>
+      -- If both the input and the stack are nonempty, we have options.
+      -- Exactly one of δ(q, a, x), δ(q, ε, x), or δ(q, a, ε) is `some`, and we have to choose the one that is `some`.
+      match
+        (M.transition (pwβ.p, AugmentEpsilon.fromChar a, AugmentEpsilon.fromChar x)),
+        (M.transition (pwβ.p, AugmentEpsilon.fromChar a, AugmentEpsilon.Epsilon)),
+        (M.transition (pwβ.p, AugmentEpsilon.Epsilon, AugmentEpsilon.fromChar x)) with
+      | some (r, y), none, none =>
+        -- If δ(q, a, x) is nonempty, we can consume a from the input,
+        -- move to the state r,
+        -- pop x from the stack,
+        -- and push y onto the stack.
+        some ⟨ r, ws, y.toList ++ xs ⟩
+      | none, some (r, y), none =>
+        -- If δ(q, ε, x) is nonempty, we can pop x from the stack,
+        -- move to the state r,
+        -- consume nothing from the input,
+        -- and push y onto the stack.
+        some ⟨ r, pwβ.w, y.toList ++ xs ⟩
+      | none, none, some (r, y) =>
+        -- If δ(q, a, ε) is nonempty, we can consume a from the input,
+        -- move to the state r,
+        -- pop nothing from the stack,
+        -- and push y onto the stack.
+        some ⟨ r, ws, y.toList ++ pwβ.β ⟩
+      | _, _, _ => none -- When the `deterministic` condition holds, this branch should never be reached.
+
+
 def Sipser_DPDA.stepTransition {Q S Γ}
   (M: Sipser_DPDA Q S Γ)
   (pwβ: Sipser_DPDA_IDesc Q S Γ)
@@ -113,3 +194,13 @@ def Sipser_DPDA.stepTransition {Q S Γ}
       | some _, none, some _   => False.elim <| by have h3 := M.deterministic pwβ.p a x; simp [exactly_one_some, hεε, hax, haε, hεx] at h3
       | none, some _, some _   => False.elim <| by have h3 := M.deterministic pwβ.p a x; simp [exactly_one_some, hεε, hax, haε, hεx] at h3
       | none, none, none       => False.elim <| by have h3 := M.deterministic pwβ.p a x; simp [exactly_one_some, hεε, hax, haε, hεx] at h3
+
+
+theorem step_in_pre_is_step_in_dpda {Q S Γ}
+  (M: Sipser_DPDA Q S Γ)
+  (idesc: Sipser_DPDA_IDesc Q S Γ) :
+  Sipser_PreDPDA.stepTransition M.pda idesc = M.stepTransition idesc := by
+  simp only [Sipser_PreDPDA.stepTransition, Sipser_DPDA.stepTransition]
+  match h2 : M.pda.transition (idesc.p, AugmentEpsilon.Epsilon, AugmentEpsilon.Epsilon) with
+  | some (r, y) => sorry
+  | none => sorry
