Dpda/Conversion/PredetToSipser.lean
@@ -210,4 +210,11 @@ def Predet_DPDA.toSipser {Q S Γ} [DecidableEq Q] (M: Predet_DPDA Q S Γ) : Sips
 theorem Predet_to_Sipser_preserves_semantics_single_step {Q S Γ}
   [Fintype Q] [DecidableEq Q] [Fintype S] [Fintype Γ] [DecidableEq Γ]
   (M: Predet_DPDA Q S Γ) (idesc: Predet_DPDA_IDesc Q S Γ) :
-  Predet_DPDA_IDesc.toSipser <$> M.stepTransition idesc = M.toSipser.stepTransition idesc.toSipser := by sorry
+  let after_step : Option (Predet_DPDA_IDesc Q S Γ) := M.stepTransition idesc
+  let after_step_sipser : Option (Sipser_DPDA_IDesc (AugmentOneState Q) S Γ) := Predet_DPDA_IDesc.toSipser <$> after_step
+  after_step_sipser = M.toSipser.stepTransition idesc.toSipser := by
+  simp [Functor.map,
+   Predet_DPDA_IDesc.toSipser,     Predet_DPDA.toSipser,
+   Predet_DPDA.stepTransition, Sipser_DPDA.stepTransition,
+  ]
+  sorry
